aarch64 ainvs: add valid_global_tables to invariants
For the proofs in ArchAInvsPre we require knowledge that the default
user-level tables do not map any user-space addresses. In hyp mode, the
default user-level table is completely empty, because the kernel has
its own separate table. We encode that empty table in the
`valid_global_tables` predicate analogously to the RISCV64 formulation.

We explicitly leave `valid_global_arch_objs` as a `typ_at` predicate,
because the proofs expect `valid_global_arch_objs` to be liftable.

Co-authored-by: Rafal Kolanski <rafal.kolanski@proofcraft.systems>
Signed-off-by: Gerwin Klein <gerwin.klein@proofcraft.systems>

proof/invariant-abstract/AARCH64/ArchInvariants_AI.thy
@@ -628,9 +628,21 @@ definition vmid_inv :: "'z::state_ext state \<Rightarrow> bool" where
 definition valid_global_arch_objs where
   "valid_global_arch_objs \<equiv> \<lambda>s. vspace_pt_at (global_pt s) s"
 
+(* global_pt is the empty default user-level vspace, corresponding to armKSGlobalUserVSpace in C.
+   On HYP platforms, the kernel has its own separate page table.
+   We need to know that the user-level table is empty so we can derive that user-level lookups
+   fail when there is no other vspace set. *)
+definition valid_global_tables_2 :: "(obj_ref \<Rightarrow> pt option) \<Rightarrow> obj_ref \<Rightarrow> bool" where
+  "valid_global_tables_2 \<equiv> \<lambda>pts global. pts global = Some (empty_pt VSRootPT_T)"
+
+locale_abbrev valid_global_tables :: "'z::state_ext state \<Rightarrow> bool" where
+  "valid_global_tables \<equiv> \<lambda>s. valid_global_tables_2 (pts_of s) (global_pt s)"
+
+lemmas valid_global_tables_def = valid_global_tables_2_def
+
 definition valid_arch_state :: "'z::state_ext state \<Rightarrow> bool" where
   "valid_arch_state \<equiv> valid_asid_table and valid_uses and vmid_inv and cur_vcpu and
-                      valid_global_arch_objs"
+                      valid_global_arch_objs and valid_global_tables"
 
 (* ---------------------------------------------------------------------------------------------- *)
 
